Syntax/Elab.lean
@@ -17,13 +17,24 @@ set_option linter.unusedVariables false
 
 open Lean Meta Elab Term Qq
 
+def assertDefEq (a b : Expr) (message : MessageData := "") : MetaM Unit := do
+  if !(<- Meta.isDefEq a b) then
+    throwError "assertDefEq failed {message}:\n{a} is not defeq to {b}"
+
 /-
   # Quotation Helpers
+  It is easy to forget what type exacle you're handling when you're just working with `Expr`,
+  and Quote4 often misbehaves.
+  Hence these helpers, to make life easier.
+  These helpers are mostly for documentation.
+  They are not rigid, and it is still possible to unsafely cast around,
+  since they're just `:= Expr` anyway.
 -/
 
 inductive ConQ where
 | nil : ConQ
-| ext : ConQ -> Name -> Expr -> ConQ
+| ext' : ConQ -> Name -> Expr -> ConQ
+| unknown : Expr -> ConQ
 def TyQ (Γ : ConQ) : Type := Expr
 def TmQ (Γ : ConQ) (A : TyQ Γ) : Type := Expr
 def VarQ (Γ : ConQ) : Type := Nat
@@ -32,12 +43,57 @@ def ConConvQ (Γ Δ : ConQ) : Type := Expr
 def TyConvQ {Γ : ConQ} (X Y : TyQ Γ) : Type := Expr
 def TmConvQ {Γ : ConQ} {A : TyQ Γ} (x y : TmQ Γ A) : Type := Expr
 
+/-- These two are definitionally equal in our metatheory, i.e. in Lean.
+  This is basically Quote4's `_ =Q _`, but behaving a bit better. -/
+def TyMDE {Γ : ConQ} (X : TyQ Γ) (Y : TyQ Γ) : Type := Unit
+
+/-- These two are definitionally equal in our metatheory, i.e. in Lean.
+  This is basically Quote4's `_ =Q _`, but behaving a bit better.
+
+  If its internal representation is `none`, it means that `X ≡ Y`.
+  If its internal representation is `some c`, it means that `c : X ≅ Y`.
+  -/
+def TmMDE {Γ : ConQ}
+  {X : TyQ Γ} {Y : TyQ Γ}
+  (x : TmQ Γ X) (y : TmQ Γ Y)
+  : Type
+  -- := Unit
+  := Option (TyConvQ X Y)
+
+@[match_pattern] def ConQ.ext : (Γ : ConQ) -> Name -> TyQ Γ -> ConQ := fun Γ name A => ConQ.ext' Γ name A
+
+def TyQ.unsafeIntro : Expr -> TyQ Γ := id
+def TmQ.unsafeIntro : Expr -> TmQ Γ A := id
+def VarQ.unsafeIntro : Nat -> VarQ Γ := id
+def SubstQ.unsafeIntro : Expr -> SubstQ Γ Δ := id
+def ConConvQ.unsafeIntro : Expr -> ConConvQ Γ Δ := id
+def TyConvQ.unsafeIntro : Expr -> TyConvQ X Y := id
+def TmConvQ.unsafeIntro : Expr -> TmConvQ x y := id
+def TyMDE.unsafeIntro : TyMDE X Y := ()
+def TmMDE.unsafeIntro : @TmMDE Γ X Y x y := none
+
+def TyQ.unsafeCast : TyQ Γ -> TyQ Γ := id
+def TmQ.unsafeCast : TmQ Γ A -> TmQ Γ' A' := id
+def VarQ.unsafeCast : VarQ Γ -> VarQ Γ' := id
+def SubstQ.unsafeCast : SubstQ Γ Δ -> SubstQ Γ' Δ' := id
+def ConConvQ.unsafeCast : ConConvQ Γ Δ -> ConConvQ Γ' Δ' := id
+def TyConvQ.unsafeCast : TyConvQ X Y -> TyConvQ X' Y' := id
+def TmConvQ.unsafeCast : TmConvQ x y -> TmConvQ x' y' := id
+def TmConvQ.unsafeCast! {x : TmQ Γ X} {y : TmQ Γ Y} : @TmConvQ Γ X x y -> TmConvQ x' y' := id
+
+-- def TyConvQ.castR : TyConvQ X Y -> TyMDE Y Z -> TyConvQ X Z := fun a b => a
+-- def TyConvQ.castL : TyMDE X Y -> TyConvQ Y Z -> TyConvQ X Z := fun a b => b
+-- def TmConvQ.castR : TmConvQ X Y -> TmMDE Y Z -> TmConvQ X Z := fun a b => a
+-- def TmConvQ.castL : TmMDE X Y -> TmConvQ Y Z -> TmConvQ X Z := fun a b => b
+-- def TmQ.cast : TyMDE A B -> TmQ Γ A -> TmQ Γ B := fun _ t => t
+
 def ConQ.quote : ConQ -> Q(Con)
 | .nil => q(Con.nil)
 | .ext Γq name Aq =>
-  let Aq : TyQ Γq := Aq
+  -- let Aq : TyQ Γq := .unsafeIntro Aq
   let Γexpr : Q(Con) := Γq.quote
   .app q(Con.ext $Γexpr) Aq
+| .unknown expr => expr
 def TyQ.quote {Γ : ConQ} (A : TyQ Γ) : Q(Ty $(Γ.quote)) := A
 def TmQ.quote {Γ : ConQ} {A : TyQ Γ} (t : TmQ Γ A) :
   have Γ : Q(Con) := Γ.quote
@@ -49,19 +105,34 @@ def SubstQ.quote (σ : SubstQ Γ Δ) :
   have Δ : Q(Con) := Δ.quote
   Q(Subst $Γ $Δ)
   := σ
+def ConConvQ.quote (c : ConConvQ Γ Δ) :
+  have Γ : Q(Con) := Γ.quote
+  have Δ : Q(Con) := Δ.quote
+  Q(ConConv $Γ $Δ) := c
 def TyConvQ.quote {Γ : ConQ} {X Y : TyQ Γ} (c : TyConvQ X Y) :
   have Γ : Q(Con) := Γ.quote
   have X : Q(Ty $Γ) := X.quote
   have Y : Q(Ty $Γ) := Y.quote
   Q(TyConv $X $Y)
   := c
+def TmConvQ.quote {Γ : ConQ} {X : TyQ Γ} {x y : TmQ Γ X} (c : @TmConvQ Γ X x y) :
+  have Γ : Q(Con) := Γ.quote
+  have X : Q(Ty $Γ) := X.quote
+  have x : Q(Tm $Γ $X) := x.quote
+  have y : Q(Tm $Γ $X) := y.quote
+  Q(TmConv $x $y)
+  := c
 
-instance : ToExpr ConQ where
-  toTypeExpr := q(Con)
-  toExpr := ConQ.quote
-instance : ToExpr (TyQ Γ) where
-  toTypeExpr := q(Ty $Γ.quote)
-  toExpr := TyQ.quote
+instance : Coe ConQ Expr where coe Γ := Γ.quote
+instance : CoeOut (TyQ Γ) Expr where coe := TyQ.quote
+instance : CoeOut (TmQ Γ A) Expr where coe := TmQ.quote
+instance : CoeOut (SubstQ Γ Δ) Expr where coe := SubstQ.quote
+instance : CoeOut (TyConvQ A B) Expr where coe := TyConvQ.quote
+instance : CoeOut (TmConvQ x y) Expr where coe := TmConvQ.quote
+
+def ConConvQ.refl : ConConvQ Γ Γ := .unsafeIntro <| mkAppN q(@ConConv.refl) #[Γ.quote]
+def ConConvQ.ext' {X Y : TyQ Γ} (c : TyConvQ X Y) : ConConvQ (.ext Γ x X) (.ext Γ y Y) :=
+  mkAppN q(@ConConv.ext') #[Γ.quote, X.quote, Y.quote, c.quote]
 
 def TyQ.U : TyQ Γ := q(@Ty.U $Γ.quote)
 def TyQ.El (t : TmQ Γ .U) : TyQ Γ := mkApp2 q(@Ty.El) Γ.quote t.quote
@@ -77,11 +148,29 @@ def SubstQ.apply (a : TmQ Γ A) : SubstQ Γ (.ext Γ name A) :=
   let a : Q(Tm $Γq $A) := a
   q(Subst.apply $a)
 
+def SubstQ.comp {Γ Θ Δ : ConQ} (δ : SubstQ Θ Δ) (σ : SubstQ Γ Θ) : SubstQ Γ Δ :=
+  have Γ : Q(Con) := Γ.quote
+  have Θ : Q(Con) := Θ.quote
+  have Δ : Q(Con) := Δ.quote
+  have δ : Q(Subst $Θ $Δ) := δ
+  have σ : Q(Subst $Γ $Θ) := σ
+  q(Subst.comp $δ $σ)
+
+def SubstQ.lift (σ : SubstQ Γ Δ) : SubstQ (Γ.ext name (W.subst σ)) (.ext Δ name W) :=
+  have Γq : Q(Con) := Γ.quote
+  have Δq : Q(Con) := Δ.quote
+  have W : Q(Ty $Δq) := W.quote
+  have σ : Q(Subst $Γq $Δq) := σ.quote
+  q(@Subst.lift $Γq $Δq $W $σ)
+
 def TmQ.app (f : TmQ Γ (.Pi name A B)) (a : TmQ Γ A) : TmQ Γ (TyQ.subst B (.apply a))
   := mkAppN q(@Tm.app) #[ Γ.quote, A.quote, B.quote, f.quote, a.quote ]
 
 def TmQ.lam {Γ name} {A : TyQ Γ} {B : TyQ (.ext Γ name A)} (body : TmQ (.ext Γ name A) B) : TmQ Γ (TyQ.Pi name A B)
   := mkAppN q(@Tm.lam) #[ Γ.quote, A.quote, B.quote, body.quote ]
+
+def TyQ.conv {Γ Δ : ConQ} (c : ConConvQ Γ Δ) (A : TyQ Γ) : TyQ Δ :=
+  mkAppN q(@Ty.conv) #[Γ.quote, Δ.quote, c.quote, A.quote]
 
 def TmQ.conv {Γ : ConQ} {X Y : TyQ Γ} (c : TyConvQ X Y) (t : TmQ Γ X) : TmQ Γ Y :=
   mkAppN q(@Tm.conv) #[Γ.quote, X.quote, Y.quote, c.quote, t.quote]
@@ -89,6 +178,7 @@ def TmQ.conv {Γ : ConQ} {X Y : TyQ Γ} (c : TyConvQ X Y) (t : TmQ Γ X) : TmQ �
 def ConQ.findVar (n : Name) : (Γ : ConQ) -> Option (VarQ Γ)
 | .nil => none
 | .ext Γ name _ => if n = name then some .zero else (Γ.findVar n).map Nat.succ
+| .unknown expr => none
 
 def VarQ.quote : {Γ : ConQ} -> (v : VarQ Γ) -> Option <| have Γ : Q(Con) := Γ.quote; ((X : Q(Ty $Γ)) × Q(Var $Γ $X))
 | .nil                   , v       => none
@@ -107,10 +197,18 @@ def VarQ.quote : {Γ : ConQ} -> (v : VarQ Γ) -> Option <| have Γ : Q(Con) := �
   let Ywki : Q(Ty (.ext $Γq $B)) := q(Ty.subst $Y .wki) -- let X : Q(Ty (.ext $Γq $Bq)) := q(@Ty.subst (.ext $Γq $Bq) $Γq $Yq (@Subst.wki $Γq $Bq))
   let vsv : Q(Var (.ext $Γq $B) $Ywki) := q(.vs $v)
   return some ⟨Ywki, vsv⟩
+| .unknown _, _ => none
 
 def TyConvQ.refl (X : TyQ Γ) : TyConvQ X X :=
   let Xq := X.quote
   q((TyConv.refl : TyConv $Xq $Xq))
+
+def TyConvQ.symm {X Y : TyQ Γ} (xy : TyConvQ X Y) : TyConvQ Y X :=
+  have Xq := X.quote
+  have Yq := Y.quote
+  have xy : Q(TyConv $Xq $Yq) := xy
+  q((TyConv.symm $xy : TyConv $Yq $Xq))
+
 def TyConvQ.trans {X Y Z : TyQ Γ} (xy : TyConvQ X Y) (yz : TyConvQ Y Z) : TyConvQ X Z :=
   have Xq := X.quote
   have Yq := Y.quote
@@ -118,10 +216,334 @@ def TyConvQ.trans {X Y Z : TyQ Γ} (xy : TyConvQ X Y) (yz : TyConvQ Y Z) : TyCon
   have xy : Q(TyConv $Xq $Yq) := xy
   have yz : Q(TyConv $Yq $Zq) := yz
   q((TyConv.trans $xy $yz : TyConv $Xq $Zq))
+
 def TyConvQ.ofEq {Γ : ConQ} :
   let Γq := Γ.quote
   {X Y : Q(Ty $Γq)} -> (prf : Q($X = $Y)) -> @TyConvQ Γ X Y
   := @fun X Y prf => q((TyConv.ofEq $prf : TyConv $X $Y))
+
+#check TyConv.Pi
+def TyConvQ.Pi {A A' : TyQ Γ}
+  {B : TyQ (.ext Γ `anomymous A)}
+  {B' : TyQ (.ext Γ `anomymous A')}
+  (Ac : TyConvQ A A')
+  -- (Bc : @TyConvQ (.ext Γ `anonymous A) B (B'.conv (.ext' Ac.symm)))
+  -- (Bc : @TyConvQ (.ext Γ `anonymous A) B B')
+  (Bc : Expr)
+  : TyConvQ (.Pi `anonymous A B) (.Pi `anonymous A' B')
+  := sorry
+
+partial def TyConvQ.isOnlyReflTransSymm (c : TyConvQ X Y) : Bool := go c
+  where go (c : Expr) : Bool :=
+    match_expr c with
+    | TyConv.refl _ _ => true
+    | TyConv.trans _ _ _ _ c1 c2 => go c1 && go c2
+    | TyConv.symm _ _ _ c => go c
+    | _ => false
+
+def TyConvQ.subst (c : @TyConvQ Δ X Y) (σ : SubstQ Γ Δ) : @TyConvQ Γ (X.subst σ) (Y.subst σ) :=
+  mkAppN q(@TyConv.subst) #[Δ.quote, Γ.quote, X, Y, c, σ]
+
+#check Ty.subst_comp
+#check TyConv.ofEq
+def TyConvQ.subst_comp {Γ Θ Δ : ConQ} {A : TyQ Δ} {σ₁ : SubstQ Θ Δ} {σ₂ : SubstQ Γ Θ}
+  : TyConvQ ((A.subst σ₁).subst σ₂) (A.subst (σ₁.comp σ₂))
+  :=
+    let eq := mkAppN q(@Ty.subst_comp) #[Γ.quote, Θ.quote, Δ.quote, A, σ₁, σ₂]
+    mkAppN q(@TyConv.ofEq) #[Γ, (A.subst σ₁).subst σ₂, A.subst (σ₁.comp σ₂), eq]
+
+def TmConvQ.refl {X : TyQ Γ} (x : TmQ Γ X) : TmConvQ x x :=
+  have Γq := Γ.quote
+  have Xq : Q(Ty $Γq) := X.quote
+  have xq : Q(Tm $Γq $Xq) := x.quote
+  q((TmConv.refl : TmConv $xq $xq))
+
+def TmConvQ.symm {T : TyQ Γ} {x y : TmQ Γ T} (xy : TmConvQ x y) : TmConvQ y x :=
+  have Γq := Γ.quote
+  have Tq : Q(Ty $Γq) := T.quote
+  have xq : Q(Tm $Γq $Tq) := x.quote
+  have yq : Q(Tm $Γq $Tq) := y.quote
+  have xy : Q(TmConv $xq $yq) := xy
+  q((TmConv.symm $xy : TmConv $yq $xq))
+
+def TmConvQ.trans {T : TyQ Γ} {x y z : TmQ Γ T} (xy : TmConvQ x y) (yz : TmConvQ y z) : TmConvQ x z :=
+  have Γq : Q(Con) := Γ.quote
+  have Tq : Q(Ty $Γq) := T.quote
+  have xq : Q(Tm $Γq $Tq) := x.quote
+  have yq : Q(Tm $Γq $Tq) := y.quote
+  have zq : Q(Tm $Γq $Tq) := z.quote
+  have xy : Q(@TmConv $Γq $Tq $xq $yq) := xy
+  have yz : Q(@TmConv $Γq $Tq $yq $zq) := yz
+  q((TmConv.trans $xy $yz : TmConv $xq $zq))
+
+-- def TmConvQ.ofEq {Γ : ConQ} :
+--   let Γq := Γ.quote
+--   {X Y : Q(Ty $Γq)} -> (prf : Q($X = $Y)) -> @TyConvQ Γ X Y
+--   := @fun X Y prf => q((TyConv.ofEq $prf : TyConv $X $Y))
+
+def TmQ.subst {A : TyQ Δ} (t : TmQ Δ A) (σ : SubstQ Γ Δ) : TmQ Γ (A.subst σ)
+  := .unsafeIntro <| mkAppN q(@Tm.subst) #[Γ.quote, Δ.quote, A, t, σ]
+
+#check TyConv.subst_lift_apply
+def TyConvQ.subst_lift_apply {σ : SubstQ Γ Δ} {B : TyQ (.ext Δ name A)}
+  : TyConvQ
+    ((B.subst (.apply a)).subst σ)
+    (TyQ.subst (TyQ.subst B (.lift σ)) (.apply (.subst a σ)))
+  := .ofEq <| (mkAppN q(@TyConv.subst_lift_apply) #[Γ, Δ, σ, A, B, a] : Expr)
+
+-- def TmHConvQ {Γ : ConQ} {X Y : TyQ Γ} (x : TmQ Γ X) (y : TmQ Γ Y) : Type := Expr
+structure TmHConvQ {Γ : ConQ} {X Y : TyQ Γ} (x : TmQ Γ X) (y : TmQ Γ Y) : Type where
+  tyConv : TyConvQ X Y
+  /-- Do not use this yourself. `TmWConv Γ.2.1 X.1 x.1 y.1` -/
+  tmConv :
+    have Γ : Q(Con) := Γ.quote
+    have X : Q(Ty $Γ) := X.quote
+    have Y : Q(Ty $Γ) := Y.quote
+    have x : Q(Tm $Γ $X) := x.quote
+    have y : Q(Tm $Γ $Y) := y.quote
+    Q(TmWConv $Γ.2.1 $X.1 $x.1 $y.1)
+
+def TmHConvQ.ofExpr (expr : Expr) : @TmHConvQ Γ X Y x y :=
+  let tyConv := mkAppN q(@TmHConv.tyConv) #[Γ, X, Y, x, y, expr]
+  let tmConv := mkAppN q(@TmHConv.tmConv) #[Γ, X, Y, x, y, expr]
+  ⟨tyConv, tmConv⟩
+
+def TmHConvQ.unsafeCast (h : TmHConvQ x y) : TmHConvQ x' y' where
+  tyConv := h.tyConv
+  tmConv := h.tmConv
+
+def TmHConvQ.ofTmConvQ (c : TmConvQ x y) : TmHConvQ x y where
+  tyConv := .refl _
+  tmConv := c
+
+def TmHConvQ.quote {X Y : TyQ Γ} {x : TmQ Γ X} {y : TmQ Γ Y} (h : TmHConvQ x y) : Expr
+  := mkAppN q(@TmHConv.mk) #[Γ.quote, X, Y, x, y, h.tyConv, h.tmConv]
+
+-- def TmHConvQ.toTyConvQ (c : @TmHConvQ Γ X Y x y) : TyConvQ X Y :=
+--   sorry
+
+def TmHConvQ.refl (x : TmQ Γ X) : TmHConvQ x x where
+  tyConv := .refl X
+  tmConv := TmConvQ.refl x
+
+def TmHConvQ.symm (xy : @TmHConvQ Γ X Y x y) : TmHConvQ y x :=
+  let tyConv := xy.tyConv.symm
+  -- have Γ : Q(Con) := Γ.quote
+  -- have X : Q(Ty $Γ) := X.quote
+  -- have Y : Q(Ty $Γ) := Y.quote
+  -- have x : Q(Tm $Γ $X) := x.quote
+  -- have y : Q(Tm $Γ $Y) := y.quote
+  let tmp := mkAppN q(@TmHConv.symm) #[Γ, X, Y, x, y, xy.quote] -- very inefficient, but for now, whatever
+  let tmp := mkAppN q(@TmHConv.tmConv) #[Γ, X, Y, x, y, tmp]
+  ⟨tyConv, tmp⟩
+
+def TmHConvQ.trans (xy : @TmHConvQ Γ X Y x y) (yz : @TmHConvQ Γ Y Z y z) : TmHConvQ x z :=
+  let tyConv := xy.tyConv |>.trans yz.tyConv
+  let tmp := mkAppN q(@TmHConv.trans) #[Γ, X, Y, Z, x, y, z, xy.quote, yz.quote] -- very inefficient...
+  let tmp := mkAppN q(@TmHConv.tmConv) #[Γ, X, Z, x, z, tmp]
+  ⟨tyConv, tmp⟩
+
+#check TmHConv.ofConvTy
+def TmHConvQ.ofConvTy (x : TmQ Γ X) (c : TyConvQ X Y) : @TmHConvQ Γ X Y x (x.conv c) where
+  tyConv := c
+  tmConv :=
+    -- see `TmHConv.ofConvTy` for a justification
+    have Γ : Q(Con) := Γ.quote
+    have X : Q(Ty $Γ) := X
+    have x : Q(Tm $Γ $X) := x
+    (mkAppN q(@TmConv.refl) #[q($Γ.2.2), q($X.2), q($x.2)] : Expr)
+
+def TmHConvQ.subst (h : @TmHConvQ Δ X Y x y) (σ : SubstQ Γ Δ)
+    : @TmHConvQ Γ _ _ (x.subst σ) (y.subst σ)
+    :=
+      let tmp := mkAppN q(@TmHConv.subst) #[Γ, Δ, X, Y, x, y, h.quote, σ]
+      let tyConv := mkAppN q(@TmHConv.tyConv) #[Γ, X.subst σ, Y.subst σ, x.subst σ, y.subst σ, tmp]
+      let tmConv := mkAppN q(@TmHConv.tmConv) #[Γ, X.subst σ, Y.subst σ, x.subst σ, y.subst σ, tmp]
+      ⟨tyConv, tmConv⟩
+
+def TmHConvQ.app_subst {Γ Δ A B f a} {σ : SubstQ Γ Δ}
+  : TmHConvQ (.subst (@TmQ.app Δ name A B f a) σ) (@TmQ.app Γ name (A.subst σ) (B.subst (.lift σ)) (f.subst σ) (a.subst σ))
+  :=
+    let tmp := mkAppN q(@TmHConv.app_subst) #[Γ, Δ, A, B, f, a, σ]
+    let args : Array Expr := #[Γ,
+        ((B.subst (.apply a)).subst σ),
+        ((B.subst σ.lift).subst (.apply (a.subst σ))),
+        ((f.app a).subst σ),
+        ((f.subst σ).app (B := B) (a.subst σ))
+      ]
+    let tyConv := mkAppN q(@TmHConv.tyConv) args
+    let tmConv := mkAppN q(@TmHConv.tmConv) args
+    ⟨tyConv, tmConv⟩
+
+attribute [irreducible] TyQ
+attribute [irreducible] TmQ
+attribute [irreducible] VarQ
+attribute [irreducible] SubstQ
+attribute [irreducible] ConConvQ
+attribute [irreducible] TyConvQ
+attribute [irreducible] TmConvQ
+attribute [irreducible] TyMDE
+attribute [irreducible] TmMDE
+
+structure IsPiResult (T : TyQ Γ) where
+  name : Name := `anonymous
+  A : TyQ Γ
+  B : TyQ (.ext Γ name A)
+  conv : TyConvQ T (TyQ.Pi name A B)
+
+partial def TyQ.isPi {Γ : ConQ} (T : TyQ Γ) : MetaM <| Option (IsPiResult T) := do
+  match_expr T with
+  | Ty.Pi Γ_ A B =>
+    have A : TyQ Γ := .unsafeIntro A
+    have B : TyQ (.ext Γ `anonymous A) := .unsafeIntro B
+    return some { A, B, conv := (TyConvQ.refl T).unsafeCast }
+  | Ty.conv _ _ _ _ => -- todo look through conv
+    throwError "TyQ.isPi: not impl for Ty.conv yet"
+  | _ => return none
+
+structure IsElResult (T : TyQ Γ) where
+  t : TmQ Γ .U
+  conv : TyConvQ T (TyQ.El t)
+
+partial def TyQ.isEl {Γ : ConQ} (T : TyQ Γ) : MetaM <| Option (IsElResult T) := do
+  match_expr T with
+  | Ty.El Γ_ t =>
+    have t : TmQ Γ .U := .unsafeIntro t
+    return some { t, conv := (TyConvQ.refl T).unsafeCast }
+  | Ty.conv _ _ _ _ => -- todo look through conv
+    throwError "TyQ.isEl: not impl for Ty.conv yet"
+  | _ => return none
+
+structure IsUResult (T : TyQ Γ) where
+  conv : TyConvQ T .U
+
+partial def TyQ.isU {Γ : ConQ} (T : TyQ Γ) : MetaM <| Option (IsUResult T) := do
+  match_expr T with
+  | Ty.U Γ_ =>
+    return some { conv := (TyConvQ.refl T).unsafeCast }
+  | Ty.conv _ _ _ _ => -- todo look through conv
+    throwError "TyQ.isU: not impl for Ty.conv yet"
+  | _ => return none
+
+structure IsAppResult (t : TmQ Γ T) where
+  name : Name := `anonymous
+  A : TyQ Γ
+  B : TyQ (.ext Γ name A)
+  f : TmQ Γ (.Pi name A B)
+  a : TmQ Γ A
+  conv : TmHConvQ t (.app f a)
+  -- mde : @TmMDE Γ T (TyQ.subst B (.apply a)) t (.app f a)
+  -- Conv : TyConvQ T (TyQ.subst B (.apply a))
+  -- -- conv : @TmConvQ Γ T t ((TmQ.app f a).conv Conv.symm) -- maybe use TmHConvQ?
+  -- conv : @TmConvQ Γ (TyQ.subst B (.apply a)) (t.conv Conv) (TmQ.app f a) -- maybe use TmHConvQ?
+partial def TmQ.isApp {Γ : ConQ} {T : TyQ Γ} (t : TmQ Γ T) : MetaM <| Option (IsAppResult t) := do
+  match_expr t with
+  | Tm.app _ A B f a =>
+    let A : TyQ Γ := .unsafeIntro A
+    let B : TyQ (.ext Γ `anonymous A) := .unsafeIntro B
+    let f : TmQ Γ (.Pi `anonymous A B) := .unsafeIntro f
+    let a : TmQ Γ A := .unsafeIntro a
+    -- have A : Q(Ty $Γ_) := A
+    -- have B : Q(Ty (.ext $Γ_ $A)) := B
+    -- have f : Q(Tm $Γ_ (.Pi $A $B)) := f
+    -- have a : Q(Tm $Γ_ $A) := a
+    -- have _prf : $T_ =Q Ty.subst $B (.apply $a) := .unsafeIntro
+    -- have _prf : $t_ =Q .app $f $a := .unsafeIntro
+    -- let tmConv : Q(TmWConv $Γ_.2.1 $T_.1 $t_.1 (.app $A.1 $B.1 $f.1 $a.1)) := q(.refl $Γ_.2.2 $T_.2 $t_.2)
+    -- let conv : TmHConvQ t (.app f a) := ⟨q(@TyConv.refl $Γ_ $T_), tmConv⟩
+    -- let Conv : TyConvQ T (TyQ.subst B (SubstQ.apply a)) := q(@TyConv.refl $Γ_ $T_)
+
+    let T_conv_Ba : TyConvQ T (TyQ.subst B (SubstQ.apply a)) := (TyConvQ.refl T).unsafeCast -- okay because `T ≡ B[a]` is defeq -- todo assign T.
+    -- todo: move the below line for `e : Expr` somewhere else
+    let e : Expr := TmConvQ.refl t |>.quote -- okay because `T ≡ B[a]` defeq and because `t ≡ .app f a` also defeq
+    let conv : @TmHConvQ Γ T (B.subst (SubstQ.apply a)) t (f.app a) := ⟨T_conv_Ba, e⟩
+    return some { A, B, f, a, conv }
+
+  | Tm.conv _ X _T X_conv_T t' =>
+    have X : TyQ Γ := .unsafeIntro X
+    have t' : TmQ Γ X := .unsafeIntro t'
+    have X_conv_T : TyConvQ X T := .unsafeIntro X_conv_T
+    let some ⟨name, A, B, f, a, conv⟩ <- TmQ.isApp t' | return none
+    let Conv : TyConvQ T (TyQ.subst B (.apply a)) := .trans X_conv_T.symm conv.tyConv
+    let h1 := TmHConvQ.ofConvTy t' X_conv_T |>.symm
+    let conv : @TmHConvQ Γ T (B.subst (SubstQ.apply a)) (t'.conv X_conv_T) (f.app a) := h1.trans conv
+    let conv : @TmHConvQ Γ T (B.subst (SubstQ.apply a)) t (f.app a) := conv.unsafeCast -- okay because `t ≡ t'.conv _` is a defeq
+    return some {
+      name := name
+      A := A
+      B := B
+      f := f
+      a := a
+      conv
+    }
+  -- | Tm.subst .. => or maybe just handle this elsewhere
+  | _ => return none
+
+structure IsLamResult (t : TmQ Γ T) where
+  name : Name := `anonymous
+  A : TyQ Γ
+  B : TyQ (.ext Γ name A)
+  body : TmQ (.ext Γ name A) B
+  Conv : TyConvQ T (.Pi name A B)
+
+partial def TmQ.isLam {Γ : ConQ} {T : TyQ Γ} (t : TmQ Γ T) : MetaM <| Option (IsLamResult t) := do
+  match_expr t with
+  | Tm.lam _ A B body =>
+    let A : TyQ Γ := .unsafeIntro A
+    let B : TyQ (.ext Γ `anonymous A) := .unsafeIntro B
+    let body : TmQ (.ext Γ `anonymous A) B := .unsafeIntro body
+    let Conv : TyConvQ T (TyQ.Pi `anonymous A B) := .unsafeCast (.refl T) -- okay because this is a defeq
+    return some { A, B, body, Conv }
+  | Tm.conv _ X __T X_conv_T t' =>
+    have X : TyQ Γ := .unsafeIntro X
+    have t' : TmQ Γ X := .unsafeIntro t'
+    have X_conv_T : TyConvQ X T := .unsafeIntro X_conv_T
+    let some {name, A, B, body, Conv := X_conv_PiAB } <- TmQ.isLam t' | return none
+    let T_conv_PiAB : TyConvQ T (.Pi name A B) := .trans X_conv_T.symm X_conv_PiAB
+    return some {
+      name
+      A
+      B
+      body
+      Conv := T_conv_PiAB
+    }
+  -- | Tm.subst .. => or maybe just handle this elsewhere
+  | _ => return none
+
+structure IsSubstTyResult (Y : TyQ Γ) where
+  Δ : ConQ
+  X : TyQ Δ
+  σ : SubstQ Γ Δ
+  conv : TyConvQ Y (X.subst σ)
+
+partial def TyQ.isSubst {Γ : ConQ} {Y : TyQ Γ} : MetaM <| Option (IsSubstTyResult Y) :=
+  match_expr Y with
+  | Ty.subst _ Δ X σ =>
+    let Δ : ConQ := .unknown Δ
+    let X : TyQ Δ := .unsafeIntro X
+    let σ : SubstQ Γ Δ := .unsafeIntro σ
+    return some { Δ, X, σ, conv := (TyConvQ.refl Y).unsafeCast } -- okay because defeq
+  -- todo look through conv
+  | _ => return none
+
+structure IsSubstTmResult (y : TmQ Γ Aσ) where
+  Δ : ConQ
+  A : TyQ Δ
+  x : TmQ Δ A
+  σ : SubstQ Γ Δ
+  -- Conv : TyConvQ Aσ (TyQ.subst A σ)
+  conv : TmHConvQ y (TmQ.subst x σ)
+
+partial def TmQ.isSubst {Γ : ConQ} {Aσ : TyQ Γ} {y : TmQ Γ Aσ} : MetaM <| Option (IsSubstTmResult y) :=
+  match_expr y with
+  | Tm.subst _ Δ A x σ =>
+    let Δ : ConQ := .unknown Δ
+    let A : TyQ Δ := .unsafeIntro A
+    let x : TmQ Δ A := .unsafeIntro x
+    let σ : SubstQ Γ Δ := .unsafeIntro σ
+    return some { Δ, A, σ, x, conv := (TmHConvQ.refl y).unsafeCast }
+  -- todo look through conv
+  | _ => return none
 
 /-
   # Reduction
@@ -131,30 +553,163 @@ def TyConvQ.ofEq {Γ : ConQ} :
   Instead, `match_expr` would be more performant and would not unfold exprs, but also a pain to write.
 
   It might also be helpful to have a dedicated reduction relation, instead of piggybacking on TyConv.
+
+  We also reduce away substitutions as far as possible.
 -/
 
-partial def TyQ.red {Γ : ConQ} (X : TyQ Γ) : MetaM <| (Y : TyQ Γ) × TyConvQ X Y := do
-  have Γq : Q(Con) := Γ.quote
-  have Xq : Q(Ty $Γq) := X
-  let cont (Y : TyQ Γ) (X_red_Y : TyConvQ X Y) : MetaM <| (Z : TyQ Γ) × TyConvQ X Z := do
-    let ⟨Z, Y_red_Z⟩ <- TyQ.red Y
-    let X_red_Z := TyConvQ.trans (X := X) X_red_Y Y_red_Z
-    return ⟨Z, X_red_Z⟩
-  match Xq with
-  | ~q(Ty.subst (Ty.subst $A $σ1) $σ2) => -- `A[σ1][σ2] = A[σ1 ∘ σ2]`
-    let Y : Q(Ty $Γq) := q(Ty.subst $A (Subst.comp $σ1 $σ2))
-    let X_red_Y : Q(TyConv $Xq $Y) := q(TyConv.ofEq Ty.subst_comp)
-    cont Y X_red_Y
-  | ~q(Ty.subst .U $σ) => -- `U[σ] ≡ U`
-    let Y : Q(Ty $Γq) := q(.U)
-    return ⟨Y, .refl X⟩
-  | ~q(Ty.subst (.El $t) $σ) => -- `(.El t)[σ] ≡ El t[σ]`
-    let Y : Q(Ty $Γq) := q(Ty.El (Tm.subst $t $σ))
-    cont Y (.refl X)
-  | ~q(Ty.subst (.Pi $A $B) $σ) => -- `(.Pi A B)[σ] ≡ Pi A[σ] B[lift σ]`
-    let Y : Q(Ty $Γq) := q(Ty.Pi (.subst $A $σ) (Ty.subst $B (.lift $σ)))
-    cont Y (.refl X)
-  | _ => return ⟨Xq, .refl X⟩ -- no-op
+-- partial def TmE.redM {γ : Q(Nat)} (t : Q(TmE $γ)) : MetaM ((t' : Q(TmE $γ)) × Q(TmERed $t $t')) := do
+--   -- withTraceNode `stx.red (myLog (f_err := fun err => return m!"TmE.red {t} ~~> ERROR {err.toMessageData}") (fun ⟨t', prf⟩ => return m!"TmE.red {t} ~~> {t'}\nProof: {prf}")) do
+--   -- withTraceNode `stx.red (niceLog m!"TmE.redM {t}") do
+--   let t₂ : Q(TmE $γ) <- whnf t
+--   have : $t =Q $t₂ := .unsafeIntro
+--   match t₂ with
+--   | ~q(TmE.app $A $B $f $a) =>
+--     let f₂ : Q(TmE $γ) <- whnf f
+--     have : $f =Q $f₂ := .unsafeIntro
+--     match f₂ with
+--     | ~q(TmE.lam $A' $B' $body) => -- have `(λ. body) a`, reduce to `body[a]`
+--       let t' : Q(TmE $γ) := q(TmE.subst $body (.cons .id $a))
+--       -- return ⟨q($t'), q(TmERed.beta)⟩
+--       let ⟨t'', prf⟩ <- TmE.redM q($t')
+--       return ⟨q($t''), q(TmERed.trans TmERed.beta $prf)⟩
+--     | _ => -- `f a ~~> f' a`
+--       let ⟨f', red⟩ <- TmE.redM q($f₂)
+--       return ⟨q(.app $A $B $f' $a), q(TmERed.app $red)⟩
+--   | _ => return ⟨t, q(.refl)⟩
+
+#check Tm.app_subst
+#check TmConv.beta
+#check Ty.Pi_subst
+
+
+mutual
+  -- Ignore the extra return type `Y` if it confuses you. Reduction works on preterms in the paper anyway.
+  partial def TmQ.red {Γ : ConQ} {X : TyQ Γ} (x : TmQ Γ X) : MetaM <| (Y : TyQ Γ) × (y : TmQ Γ Y) × TmHConvQ x y := do
+    let cont {Y} (y : TmQ Γ Y) (x_red_y : TmHConvQ x y) : MetaM <| (Z : TyQ Γ) × (z : TmQ Γ Z) × TmHConvQ x z := do
+      let ⟨Z, z, y_red_z⟩ <- TmQ.red y
+      let x_red_z := TmHConvQ.trans (Γ := Γ) (x := x) x_red_y y_red_z
+      return ⟨Z, z, x_red_z⟩
+    if let .some ⟨Δ, C, t, σ, x_conv_tσ⟩ <- x.isSubst then
+      -- `x ≡ t[σ] : C[σ]` with `T ≡ C[σ]`
+      -- let x_mde : TmMDE x (TmQ.subst t σ) := .unsafeIntro
+      if let .some ⟨name, A, B, f, a, t_conv_app⟩ <- t.isApp then
+        -- `t ≡ .app f a` of type `B[apply a]`
+        -- `x ≡ (.app f a)[σ]` of type `B[apply a][σ]`
+        -- with Conv : `C ≅ B[apply a]`
+        let Aσ := TyQ.subst A σ
+        let Bσ := TyQ.subst B σ.lift
+        let fσ : TmQ Γ ((TyQ.Pi name A B).subst σ) := TmQ.subst f σ
+        let fσ : TmQ Γ (TyQ.Pi name (A.subst σ) (B.subst σ.lift)) := fσ.unsafeCast -- okay because `(Pi A B)[σ] ≡ Pi A[σ] B[lift σ]` is a defeq, see `Ty.Pi_subst`
+        let aσ := TmQ.subst a σ
+
+        let Y := TyQ.subst (TyQ.subst B (.lift σ)) (.apply (.subst a σ))
+        let y : TmQ Γ Y := .app fσ aσ -- `.app f[σ] a[σ]` of type `B[lift σ][apply a[σ]]`
+
+        let prf := t_conv_app.subst σ -- `t[σ] ≅ (app f a)[σ]`
+        let prf := x_conv_tσ |>.trans prf -- `x ≅ (app f a)[σ]`
+        let prf := prf |>.trans TmHConvQ.app_subst
+
+        return <- cont y prf
+    return ⟨X, x, .refl x⟩
+    -- sorry
+    -- match_expr x with -- `Γ ⊢ x : T`
+    -- | Tm.subst _ Δ C t σ =>
+    --   -- `Γ ⊢ t[σ] : C[σ]` with `T ≡ C[σ]` and `x ≡ t[σ]`, with `Δ ⊢ t : C`
+    --   have Δ : ConQ := .unknown Δ
+    --   have C : TyQ Δ := .unsafeIntro C
+    --   have t : TmQ Δ C := .unsafeIntro t
+    --   have σ : SubstQ Γ Δ := .unsafeIntro σ
+    --   match_expr t with -- `Δ ⊢ t : C`
+    --   | Tm.app _ A B f a => -- ** `(f a)[σ] = (f[σ] a[σ])` : `B[lift σ][apply a[σ]]` by Tm.app_subst
+    --     -- ? problem: `B[apply a][σ]` is only propEq to `B[lift σ][apply a[σ]]`, not defeq in metatheory.
+    --     -- `Δ ⊢ (f a) : B[apply a]` with `C ≡ B[apply a]`
+    --     have A : Q(Ty $Δ) := A
+    --     have B : Q(Ty (.ext $Δ $A)) := B
+    --     have f : Q(Tm $Δ (.Pi $A $B)) := f
+    --     have a : Q(Tm $Δ $A) := a
+    --     have Aσ : Q(Ty $Γ_) := q(Ty.subst $A $σ)
+    --     have _prf : $Aσ =Q (Ty.subst $A $σ) := .unsafeIntro
+    --     have Bσ : Q(Ty (.ext $Γ_ $Aσ)) := q(Ty.subst $B (Subst.lift (W := $A) $σ))
+    --     have _prf : $Bσ =Q Ty.subst $B (Subst.lift (W := $A) $σ) := .unsafeIntro
+    --     have fσ : Q(Tm $Γ_ (.Pi $Aσ $Bσ)) := q(Tm.subst $f $σ)
+    --     have aσ : Q(Tm $Γ_ $Aσ) := q(Tm.subst $a $σ)
+    --     have x : Q(Tm $Γ_ (Ty.subst (Ty.subst $B (.apply $a)) $σ)) := x
+    --     have y : Q(Tm $Γ_ (Ty.subst $Bσ (.apply $aσ))) := q(@Tm.app $Γ_ $Aσ $Bσ $fσ $aσ)
+    --     have typeConv : Q(TyConv (Ty.subst $Bσ (.apply $aσ)) (Ty.subst (Ty.subst $B (.apply $a)) $σ) )
+    --       := q(.ofEq sorry) -- todo
+    --     have y : Q(Tm $Γ_ (Ty.subst (Ty.subst $B (.apply $a)) $σ)) := q(Tm.conv $typeConv $y)
+    --     have x_red_y : Q(TmConv $x $y)
+    --       -- := q(TmConv.ofEq Tm.app_subst) -- todo
+    --       := q(sorry)
+    --     cont y x_red_y
+    --   | _ => return ⟨x, .refl x⟩
+    -- | Tm.app _ A B f a =>
+    --   -- `Γ ⊢ f a : B[apply a]` with `T ≡ B[apply a]`
+    --   have A : Q(Ty $Γ_) := A
+    --   have B : Q(Ty (.ext $Γ_ $A)) := B
+    --   have f : Q(Tm $Γ_ (.Pi $A $B)) := f
+    --   have a : Q(Tm $Γ_ $A) := a
+    --   have _prf : $T_ =Q Ty.subst $B (.apply $a) := .unsafeIntro
+    --   match_expr f with
+    --   | Tm.lam _ _A _B body => -- ** beta reduction: `Γ ⊢ .app (.lam body) a ≅ body[apply a] : B[apply a]`
+    --     have body : Q(Tm (.ext $Γ_ $A) $B) := body
+    --     let y : Q(Tm $Γ_ (Ty.subst $B (.apply $a))) := q(Tm.subst $body (.apply $a))
+    --     let x_red_y : Q(TmConv (.app (.lam $body) $a) $y) := q(TmConv.beta $body $a)
+    --     cont y x_red_y
+    --   | _ => return ⟨x, .refl x⟩
+    -- | _ => return ⟨x, .refl x⟩
+
+  partial def TyQ.red {Γ : ConQ} (X : TyQ Γ) : MetaM <| (Y : TyQ Γ) × TyConvQ X Y := do
+    let cont (Y : TyQ Γ) (X_red_Y : TyConvQ X Y) : MetaM <| (Z : TyQ Γ) × TyConvQ X Z := do
+      let ⟨Z, Y_red_Z⟩ <- TyQ.red Y
+      let X_red_Z := TyConvQ.trans (X := X) X_red_Y Y_red_Z
+      return ⟨Z, X_red_Z⟩
+
+    if let some ⟨Θ, X', σ1, conv⟩ <- X.isSubst then
+      if let some ⟨Δ, X'', σ2, conv₂⟩ <- X'.isSubst then
+        -- `X''[σ2][σ1] = X''[σ2 ∘ σ1]`
+        let σ := SubstQ.comp σ2 σ1
+        let Y := TyQ.subst X'' σ
+        have prf : @TyConvQ Γ ((X''.subst σ2).subst σ1) Y := .subst_comp
+        have tmp := conv₂.subst σ1
+        have tmp := conv.trans tmp
+        return <- cont Y (tmp.trans prf)
+
+    if let some ⟨Δ, X', σ, conv1⟩ <- X.isSubst then
+      if let some ⟨conv2⟩ <- X'.isU then
+        let Y := @TyQ.U Γ -- `U[σ] ≡ U`
+        return <- cont TyQ.U sorry
+      if let some ⟨name, A, B, conv⟩ <- X'.isPi then
+        sorry
+      if let some ⟨t, conv⟩ <- X'.isEl then
+        let y : TmQ Γ (.subst .U σ) := t.subst σ
+        let y : TmQ Γ .U := y.unsafeCast -- okay because this is a defeq
+        return ⟨TyQ.El y, sorry⟩
+
+    return ⟨X, .refl X⟩
+
+    -- have Γq : Q(Con) := Γ.quote
+    -- have Xq : Q(Ty $Γq) := X
+    -- let cont (Y : TyQ Γ) (X_red_Y : TyConvQ X Y) : MetaM <| (Z : TyQ Γ) × TyConvQ X Z := do
+    --   let ⟨Z, Y_red_Z⟩ <- TyQ.red Y
+    --   let X_red_Z := TyConvQ.trans (X := X) X_red_Y Y_red_Z
+    --   return ⟨Z, X_red_Z⟩
+    -- match Xq with
+    -- | ~q(Ty.subst (Ty.subst $A $σ1) $σ2) => -- `A[σ1][σ2] = A[σ1 ∘ σ2]`
+    --   let Y : Q(Ty $Γq) := q(Ty.subst $A (Subst.comp $σ1 $σ2))
+    --   let X_red_Y : Q(TyConv $Xq $Y) := q(TyConv.ofEq Ty.subst_comp)
+    --   cont Y X_red_Y
+    -- | ~q(Ty.subst .U $σ) => -- `U[σ] ≡ U`
+    --   let Y : Q(Ty $Γq) := q(.U)
+    --   return ⟨Y, .refl X⟩
+    -- | ~q(Ty.subst (.El $t) $σ) => -- `(.El t)[σ] ≡ El t[σ]` (todo: insert ofEq proof anyway, to help lean unifier?)
+    --   let Y : Q(Ty $Γq) := q(Ty.El (Tm.subst $t $σ))
+    --   cont Y (.refl X)
+    -- | ~q(Ty.subst (.Pi $A $B) $σ) => -- `(.Pi A B)[σ] ≡ Pi A[σ] B[lift σ]`
+    --   let Y : Q(Ty $Γq) := q(Ty.Pi (.subst $A $σ) (Ty.subst $B (.lift $σ)))
+    --   cont Y (.refl X)
+    -- | _ => return ⟨Xq, .refl X⟩ -- no-op
+
 
   /- The Quote4 match arms above do something like this, iirc:
     let Δ : Q(Con) <- mkFreshExprMVarQ q(Con)
@@ -186,23 +741,163 @@ partial def TyQ.red {Γ : ConQ} (X : TyQ Γ) : MetaM <| (Y : TyQ Γ) × TyConvQ 
       | _ => sorry
     | _ => sorry
   -/
+end
 
 /-
   # Typed Algorithmic Conversion Checking
 -/
 
+-- /-- Strips `Ty.conv`s.
+--   Given a `Ty.conv c X : Ty Γ`, return just `X : Ty Δ` for some other context.
+--   We still pretend that we return `X : Ty Γ`, which is wrong! But, in `Ty.isDefEqRed` we ignore
+--   contexts, and so this is okay.
+--   Due to `c : Γ ≅ Δ` we still have `Ty Γ = Ty Δ`, but since Lean is an intensional type theory,
+--   we need the conversion cast.
+-- -/
+-- private partial def TyQ.stripConv (X : TyQ Γ) : TyQ Γ :=
+--   match_expr X with
+--   | Ty.conv _ _ _ X => TyQ.stripConv X
+--   | _ => X
+-- private partial def TmQ.stripConv (t : TmQ Γ X) : TmQ Γ X :=
+--   match_expr t with
+--   | Tm.conv _ _ _ _ t => TmQ.stripConv t
+--   | _ => t
+
+#check TmWConv.app
+
+structure TmQ.InferRedResult (x : TmQ Γ X) (y : TmQ Γ Y) where
+  /-- The inferred pre-reduced type. -/
+  T : TyQ Γ
+  T_conv_X : TyConvQ T X
+  T_conv_Y : TyConvQ T Y
+  conv : TmHConvQ x y
+
+structure TmQ.InferResult (x : TmQ Γ X) (y : TmQ Γ Y) where
+  conv : TmHConvQ x y
+
+#check Ty.Pi.inj
+def TyQ.Pi_inj (c : @TyConvQ Γ (.Pi a1 A₁ B₁) (.Pi a2 A₂ B₂))
+  : (Ac : @TyConvQ Γ A₁ A₂) × @TyConvQ (.ext Γ a1 A₁) B₁ (B₂.conv (ConConvQ.ext' Ac.symm))
+  := sorry
+
 mutual
-  /-- `Γ ⊢ t ~ t' |> T`. The `out_T` here is an output, and should be a metavariable. -/
-  partial def TmQ.infer (out_T : TyQ Γ) (x y : TmQ Γ out_T) : MetaM (TmConvQ x y) :=
-    sorry
+  -- /-- `Γ ⊢ t ~ₕ t' |> T` Neutral terms are comparable, inferring the *reduced* type T.
+  --   The `out_T` here is an output, and should be a metavariable. -/
+  -- partial def TmQ.inferRed (out_T : TyQ Γ) (x y : TmQ Γ out_T) : MetaM (TmHConvQ x y) := do
+  --   throwError "TmQ.inferRed: not yet implemented"
 
-  /-- `Γ ⊢ x ≅ y <| T` -/
-  partial def TmQ.isDefEq (T : TyQ Γ) (x y : TmQ Γ T) : MetaM (TmConvQ x y) :=
-    sorry
+  /-- `Γ ⊢ t ~ₕ t' |> T` Neutral terms are comparable, inferring the *reduced* type T. -/
+  -- partial def TmQ.inferRed (x : TmQ Γ out_X) (y : TmQ Γ out_Y) : MetaM (@TmHConvQ Γ out_X out_Y x y) := do
+  partial def TmQ.inferRed (x : TmQ Γ out_X) (y : TmQ Γ out_Y) : MetaM (TmQ.InferRedResult x y) := do
+    throwError "TmQ.inferRed: not yet implemented"
 
-  /-- `Γ ⊢ X ≅ Y <|` -/
-  partial def TyQ.isDefEq (X Y : TyQ Γ) : MetaM (TyConvQ X Y) :=
-    sorry
+  -- /-- `Γ ⊢ t ~ t' |> T` Neutral terms are comparable, inferring type T.
+  --   The `out_T` here is an output, and should be a metavariable. -/
+  -- partial def TmQ.infer (out_T : TyQ Γ) (x y : TmQ Γ out_T) : MetaM (TmHConvQ x y) := do
+
+  /-- `Γ ⊢ x ~ y |> X` Neutral terms are comparable, inferring type X. -/
+  partial def TmQ.infer (x : TmQ Γ out_X) (y : TmQ Γ out_Y) : MetaM (TmHConvQ x y) := do
+    have Γq : Q(Con) := Γ.quote
+    if let some ⟨name1, A1, B1, n, u, Conv⟩ <- x.isApp then
+      if let .some ⟨name2, A2, B2, n', u', Conv'⟩ <- y.isApp then
+        -- __NApp__
+        let ⟨T, T_conv_idk, T_conv_idk2, conv⟩ <- TmQ.inferRed n n'
+        let some ⟨name, A, B, T_conv_PiAB⟩ <- T.isPi | throwError "TmQ.infer: NApp case, inferRed returned {T.quote} which is not a Pi"
+        let A1c : TyConvQ A1 A := sorry
+        let A2c : TyConvQ A2 A := sorry
+        let B1c : TyConvQ B1 (B.conv (.ext' A1c.symm)) := sorry
+        let B2c : TyConvQ B2 (B.conv (.ext' A2c.symm)) := sorry
+        -- let n : TmQ Γ (.Pi name A B) := n.unsafeCast
+        -- let n' : TmQ Γ (.Pi name A B) := n'.unsafeCast
+        -- let u : TmQ Γ A := u.unsafeCast
+        -- let u' : TmQ Γ A := u'.unsafeCast
+
+        let u_conv_u' <- TmQ.isDefEq A (u.conv A1c) (u'.conv A2c)
+        let .true <- Meta.isDefEq out_T (TyQ.subst B (.apply u)) | throwError "TmQ.infer: Failed to assign {out_T.quote}" -- assign `out_T` := `B[u]`
+        let prf : TmConvQ x y := q((sorry : @TmConv $Γq ))
+        return sorry
+    throwError "{Expr.const `TmQ.infer []}: Don't know how to handle\n  {x.quote}\n~\n  {y.quote}\n|>\n  {out_T.quote}"
+
+  -- partial def TmE.isDefEqM {γ : Q(Nat)} (Γ : Q(ConE $γ)) (X : Q(TyE $γ)) (x₁ x₂ : Q(TmE $γ)) : MetaM Q(TmEDefEq $Γ $X $x₁ $x₂) := do
+  --   -- withTraceNode `stx.isDefEq (niceLog m!"TmE.isDefEqM (X:={X}): checking\n  {x₁}\n≅ {x₂}\n") do
+  --   let ⟨X', X_red⟩ <- TyE.redM X
+  --   let ⟨x₁', x₁_red⟩ <- TmE.redM x₁
+  --   let ⟨x₂', x₂_red⟩ <- TmE.redM x₂
+  --   match X' with
+  --   | ~q(.Pi $A $B) => -- __negative__: Want `Γ ⊢ x₁ ≅ₕ x₂ : Pi A B`, so do η-expansion
+  --     let x_eta : Q(TmE ($γ + 1)) := q(TmE.app (TyE.subst $A .wki) (TyE.subst $B (.lift .wki)) (TmE.subst $x₁' .wki) (.var .vz))
+  --     let y_eta : Q(TmE ($γ + 1)) := q(TmE.app (TyE.subst $A .wki) (TyE.subst $B (.lift .wki)) (TmE.subst $x₂' .wki) (.var .vz))
+  --     let prf   : Q(TmEDefEq (.ext $Γ $A) $B $x_eta $y_eta) <- TmE.isDefEqM q(.ext $Γ $A) q($B) q($x_eta) q($y_eta)
+  --     let prf'  : Q(TmEDefEq $Γ (.Pi $A $B) $x₁' $x₂') := q(TmEDefEq.eta $prf)
+  --     let prf'' : Q(TmEDefEq $Γ $X $x₁ $x₂) := q(TmEDefEq.red_cert $X_red $x₁_red $x₂_red $prf')
+  --     return prf''
+  --   | ~q(.U) =>
+  --     match x₁', x₂' with
+  --     | ~q(.pi $A $B), ~q(.pi $A' $B') => -- __positive-canonical__: Want `Γ ⊢ Pi A B ≅ₕ Pi A' B' : U`, so use Pi-congr
+  --       let A_defeq_A' <- TmE.isDefEqM Γ q(.U) q($A) A'
+  --       let B_defeq_B' <- TmE.isDefEqM q(.ext $Γ $A) q(.U) B B'
+  --       let prf := q(TmEDefEq.congr_pi $A_defeq_A' $B_defeq_B')
+  --       return q(TmEDefEq.red_cert $X_red $x₁_red $x₂_red $prf)
+  --     | _, _ => -- __positive-neutral__: From `Γ ⊢ x₁ ~ x₂ |> Y` and `Ty₊ X` conclude `Γ ⊢ x₁ ≅ x₂ <| X`.
+  --       let ⟨Y, prf⟩ <- TmE.inferM Γ x₁' x₂' -- and Y must necessarily be convertible to X'
+  --       -- let d : Q(TyWConv $Γ $X' $Y) := q(sorry)
+  --       -- throwError "TmE.isDefEqM: pos-neu not yet implemented"
+  --       return q(TmEDefEq.red_cert $X_red $x₁_red $x₂_red <| TmEDefEq.neu_inf (B := $Y) (A := $X') $prf)
+  --     | _, _ => throwError "TmE.isDefEqM: type-case .U: Don't know how to match x₁'={x₁'}, x₂'={x₂'}"
+  --   | _ => throwError "TmE.isDefEqM: Don't know how to match X'={X'}"
+
+  /-- `Γ ⊢ x ≅ₕ y <| T` Reduced terms are convertible at type T. -/
+  partial def TmQ.isDefEqRed (T : TyQ Γ) (x y : TmQ Γ T) : MetaM (TmHConvQ x y) := do
+    have Γq : Q(Con) := Γ.quote
+    have Tq : Q(Ty $Γq) := T.stripConv -- stripConv is dangerous
+    have xq : Q(Tm $Γq $Tq) := x.stripConv -- stripConv is dangerous
+    have yq : Q(Tm $Γq $Tq) := y.stripConv -- stripConv is dangerous
+    match Tq with
+    -- | ~q(Ty.Pi $A $B) => -- __negative__: Want `Γ ⊢ x₁ ≅ₕ x₂ : Pi A B`, so do η-expansion
+    --   sorry
+    | ~q(Ty.U) => -- __NeuPos__
+      let S : Q(Ty $Γq) <- mkFreshExprMVarQ q(Ty $Γq)
+      let x_conv_y : TmConvQ x y <- @TmQ.infer Γ S x y
+      return x_conv_y
+    | _ => throwError "{Expr.const `TmQ.isDefEqRed []}: Don't know how to handle\n  {xq}\n≅ₕ\n  {yq}\n<|\n  {Tq}"
+    -- match xq, yq with
+    -- | _, _ => throwError "{Expr.const `TmQ.isDefEqRed []}: Don't know how to handle\n  {xq}\n≅ₕ\n  {yq}\n<|\n  {Tq}"
+
+  /-- `Γ ⊢ X ≅ₕ Y <|` Reduced types are convertible. -/
+  partial def TyQ.isDefEqRed (X Y : TyQ Γ) : MetaM (TyConvQ X Y) := do
+    have Γq : Q(Con) := Γ.quote
+    have Xq : Q(Ty $Γq) := X.stripConv -- stripConv is dangerous
+    have Yq : Q(Ty $Γq) := Y.stripConv -- stripConv is dangerous
+    match Xq, Yq with -- What if we encounter a `.conv`? We can ignore it in this case, because this algorithm never looks at the context (the context is (almost) only there for documentation purposes).
+    | ~q(Ty.U), ~q(Ty.U) => return TyConvQ.refl X
+    | ~q(.Pi $A₁ $B₁), ~q(.Pi $A₂ $B₂) =>
+      let dA <- @TyQ.isDefEq Γ A₁ A₂
+      let c : ConConvQ (.ext Γ `anonymous A₂) (.ext Γ `anonymous A₁) := ConConvQ.ext' (.symm dA)
+      let B₂  : TyQ (.ext Γ `anonymous A₂) := B₂
+      let B₂' : TyQ (.ext Γ `anonymous A₁) := TyQ.conv c B₂ -- ? For this algorithm, we don't need .conv actually, right?
+      let dB <- @TyQ.isDefEq (ConQ.ext Γ `anonymous A₁) B₁ B₂'
+      let e /- : `Γ ⊢ .Pi A₁ B₁ ≅ .Pi A₂ (B₂.conv _)` -/ := mkAppN q(@TyConv.Pi) #[Γq, A₁, A₂, B₁, B₂', dA, dB]
+      return e
+    | ~q(.El $t₁), ~q(.El $t₂) =>
+      let dt <- @TmQ.isDefEq Γ TyQ.U t₁ t₂
+      return mkAppN q(@TyConv.El) #[Γ.quote, t₁, t₂, dt]
+    | _ => throwError m!"{Expr.const `TyQ.isDefEqRed []}: Don't know how to handle {Xq} ≅ₕ {Yq}"
+    -- | _ => throwError "TyQ.isDefEqRed: Don't know how to handle {Xq} ≅ₕ {Yq}"
+
+  /-- `Γ ⊢ x ≅ y <| T` Terms are convertible at type T. -/
+  partial def TmQ.isDefEq (T : TyQ Γ) (x y : TmQ Γ T) : MetaM (TmHConvQ x y) := do
+    let ⟨X, xr, x_red_xr⟩ <- TmQ.red x
+    let ⟨Y, yr, y_red_yr⟩ <- TmQ.red y
+    let xr_conv_yr <- TmQ.isDefEqRed T xr yr
+    return .trans (.trans x_red_xr xr_conv_yr) (.symm y_red_yr)
+
+  /-- `Γ ⊢ X ≅ Y <|` Types are convertible. -/
+  partial def TyQ.isDefEq (X Y : TyQ Γ) : MetaM (TyConvQ X Y) := do
+    -- ? Here, we want to reduce away substitutions, but not necessarily conversion stuff.
+    let ⟨Xr, X_red_Xr⟩ <- TyQ.red X
+    let ⟨Yr, Y_red_Yr⟩ <- TyQ.red Y
+    let Xr_conv_Yr <- TyQ.isDefEqRed Xr Yr
+    return TyConvQ.trans (TyConvQ.trans X_red_Xr Xr_conv_Yr) (TyConvQ.symm Y_red_Yr)
 end
 
 /-
@@ -298,7 +993,7 @@ mutual
     if <- Meta.isDefEq A' A then -- This `Meta.isDefEq` is only an optimization to avoid needless `Tm.conv`
       return t
     else
-      let c : @TyConvQ Γ A' A := q((sorry : TyConv $A'.quote $A.quote)) -- todo: try finding conversion proof
+      let c : @TyConvQ Γ A' A <- TyQ.isDefEq A' A
       return TmQ.conv c t
 end
 
