Syntax/Experiments/Unification.lean
@@ -1,0 +1,13 @@
+import Aesop
+import Qq
+import Lean
+import Syntax.Erased
+import Syntax.Wellformed
+import Syntax.AllTogether
+import Syntax.Elab
+
+set_option pp.fieldNotation.generalized false
+
+open Notation
+
+#check Ty(Type -> Type)
